Added model state initialization

poSTVM/poSTVM_initializer.thy
@@ -2,8 +2,6 @@ theory poSTVM_initializer
   imports poSTVM_state_alt
 begin
 
-
-
 fun exec_sev_expr :: "nat \<Rightarrow> expr_stack \<Rightarrow> model_state \<Rightarrow> (basic_post_type option) list" where
   "exec_sev_expr 0 _ st = [None]"
 | "exec_sev_expr (Suc n) [] st = [None]"
@@ -28,12 +26,15 @@ fun exec_sev_expr :: "nat \<Rightarrow> expr_stack \<Rightarrow> model_state \<R
 (*TO DO Function Call*)
 | "exec_sev_expr (Suc n) ((expr_op.FunctionCall v1 v2)#other) st  =
   None#(exec_sev_expr n other st)" 
+declare exec_sev_expr.simps [simp]
+declare exec_sev_expr.elims [elim]
 
-fun exec_expr :: "expr_stack \<Rightarrow> model_state \<Rightarrow> basic_post_type option" where
+definition exec_expr :: "expr_stack \<Rightarrow> model_state \<Rightarrow> basic_post_type option" where
  "exec_expr st model_st = nth (exec_sev_expr 1 st model_st) 0"
+declare exec_expr_def [simp]
 
 text "Initialization of array"
-fun initialize_array :: "model_state \<Rightarrow> stacked_var_init \<Rightarrow> stacked_var_init" where
+definition initialize_array :: "model_state \<Rightarrow> stacked_var_init \<Rightarrow> stacked_var_init" where
 "initialize_array st var= 
   (case var of 
     (stacked_var_init.Array interval values (Some expr_list)) \<Rightarrow> 
@@ -56,43 +57,45 @@ fun initialize_array :: "model_state \<Rightarrow> stacked_var_init \<Rightarrow
             (stacked_array_interval.Int int1 int2)) 
         values 
         None))"
+declare initialize_array_def [simp]
 
 text "Initialization of symbolic variable"
-fun initialize_symbolic :: "model_state \<Rightarrow> stacked_var_init  \<Rightarrow> stacked_var_init" where
+definition initialize_symbolic :: "model_state \<Rightarrow> stacked_var_init  \<Rightarrow> stacked_var_init" where
 "initialize_symbolic st var= 
   (case var of
     (stacked_var_init.Symbolic value (Some init_stack)) \<Rightarrow> 
       (stacked_var_init.Symbolic (the (exec_expr init_stack st)) None) |
     (stacked_var_init.Symbolic value None) \<Rightarrow> 
       (stacked_var_init.Symbolic value None))"
+declare initialize_symbolic_def [simp]
 
 (*TO DO FunctionBlock init*)
 text "Initialization of stacked var"
-fun initialize_stacked_vars :: "model_state \<Rightarrow> stacked_vars \<Rightarrow> stacked_vars" where
-"initialize_stacked_vars st vars =
-  (fmmap
-    (\<lambda>init.
-      (case init of
-        (stacked_var_init.Symbolic value init_option) \<Rightarrow> (initialize_symbolic st init) |
-        (stacked_var_init.Array interval values init_option) \<Rightarrow> (initialize_array st init) |
-        (stacked_var_init.FunctionBlock name) \<Rightarrow> (stacked_var_init.FunctionBlock name)) )
-    vars) "
+definition initialize_stacked_var :: "model_state \<Rightarrow> stacked_var_init \<Rightarrow> stacked_var_init" where
+"initialize_stacked_var st var =
+  (case var of
+        (stacked_var_init.Symbolic value init_option) \<Rightarrow> (initialize_symbolic st var) |
+        (stacked_var_init.Array interval values init_option) \<Rightarrow> (initialize_array st var) |
+        (stacked_var_init.FunctionBlock name) \<Rightarrow> (stacked_var_init.FunctionBlock name)) "
+declare initialize_stacked_var_def [simp]
 
 text "Initialization of proc_vars"
 definition initialize_stacked_proc_vars :: "model_state \<Rightarrow> stacked_proc_vars \<Rightarrow> stacked_proc_vars" where
-"initialize_stacked_proc_vars st (proc_var#other) = 
-  ((case proc_var of
-    (stacked_proc_var.Var stacked_vars) \<Rightarrow> (stacked_proc_var.Var (initialize_stacked_vars st stacked_vars))|
-    (stacked_proc_var.ProcessVar var) \<Rightarrow> (stacked_proc_var.ProcessVar var)|
-    (stacked_proc_var.InOutVar stacked_vars) \<Rightarrow> (stacked_proc_var.InOutVar (initialize_stacked_vars st stacked_vars)) |
-    (stacked_proc_var.InVar stacked_vars) \<Rightarrow> (stacked_proc_var.InVar (initialize_stacked_vars st stacked_vars))|
-    (stacked_proc_var.OutVar stacked_vars) \<Rightarrow> (stacked_proc_var.OutVar (initialize_stacked_vars st stacked_vars)))
-  #(initialize_stacked_proc_vars st other))"
+"initialize_stacked_proc_vars st vars = 
+  (fmmap_keys
+    (\<lambda>name var. (case var of
+                  stacked_proc_var.Var val \<Rightarrow> (stacked_proc_var.Var (initialize_stacked_var st val))
+                | stacked_proc_var.ProcessVar val \<Rightarrow> (stacked_proc_var.ProcessVar val)
+                | stacked_proc_var.InOutVar val \<Rightarrow> (stacked_proc_var.InOutVar (initialize_stacked_var st val))
+                | stacked_proc_var.InVar val \<Rightarrow> (stacked_proc_var.InVar (initialize_stacked_var st val))
+                | stacked_proc_var.OutVar val \<Rightarrow> (stacked_proc_var.OutVar (initialize_stacked_var st val)) ))
+    vars)"
+declare initialize_stacked_proc_vars_def [simp]
 
-(*TO DO*)
 text "Initialization of process variables"
-fun initialize_process_vars :: "model_state \<Rightarrow> model_state" where
-"initialize_process_vars (model_state.ST global_vars_list (program_map,cur_prog_name) fb_decl_list f_decl_list) =
+definition initialize_process_vars :: "model_state \<Rightarrow> model_state" where
+"initialize_process_vars st =
+  (case st of (model_state.ST global_vars_list (program_map,cur_prog_name) fb_decl_list f_decl_list) \<Rightarrow>
   (let st = (model_state.ST global_vars_list (program_map,cur_prog_name) fb_decl_list f_decl_list) 
   in  (model_state.ST 
     global_vars_list 
@@ -107,25 +110,27 @@ fun initialize_process_vars :: "model_state \<Rightarrow> model_state" where
        program_map,
       cur_prog_name) 
     fb_decl_list 
-    f_decl_list))"
+    f_decl_list)))"
+declare initialize_process_vars_def [simp]
 
 text "Initialization of prog_vars"
-fun initialize_stacked_prog_vars :: "model_state \<Rightarrow> stacked_prog_var list \<Rightarrow> stacked_prog_var list" where
-"initialize_stacked_prog_vars _ [] = []" |
-"initialize_stacked_prog_vars st (prog_var#other) = 
-  ((case prog_var of
-    (stacked_prog_var.ExtVar stacked_vars) \<Rightarrow> (stacked_prog_var.ExtVar (initialize_stacked_vars st stacked_vars))|
-    (stacked_prog_var.Var stacked_vars) \<Rightarrow> (stacked_prog_var.Var (initialize_stacked_vars st stacked_vars))|
-    (stacked_prog_var.InOutVar stacked_vars) \<Rightarrow> (stacked_prog_var.InOutVar (initialize_stacked_vars st stacked_vars))|
-    (stacked_prog_var.InVar stacked_vars) \<Rightarrow> (stacked_prog_var.InVar (initialize_stacked_vars st stacked_vars))|
-    (stacked_prog_var.OutVar stacked_vars) \<Rightarrow> (stacked_prog_var.OutVar (initialize_stacked_vars st stacked_vars)))
-   #(initialize_stacked_prog_vars st other))"
+definition initialize_stacked_prog_vars :: "model_state \<Rightarrow> stacked_prog_vars \<Rightarrow> stacked_prog_vars" where
+"initialize_stacked_prog_vars st vars = 
+  (fmmap
+    (\<lambda>var. (case var of
+             stacked_prog_var.Var val \<Rightarrow> (stacked_prog_var.Var (initialize_stacked_var st val))
+           | stacked_prog_var.ExtVar val \<Rightarrow> (stacked_prog_var.ExtVar (initialize_stacked_var st val))
+           | stacked_prog_var.InOutVar val \<Rightarrow> (stacked_prog_var.InOutVar (initialize_stacked_var st val))
+           | stacked_prog_var.InVar val \<Rightarrow> (stacked_prog_var.InVar (initialize_stacked_var st val))
+           | stacked_prog_var.OutVar val \<Rightarrow> (stacked_prog_var.OutVar (initialize_stacked_var st val)) ))
+    vars)"
+declare initialize_stacked_prog_vars_def [simp]
 
-(*TO DO*)
 text "Initialization of program variables"
-fun initialize_program_vars :: "model_state \<Rightarrow> model_state" where
-"initialize_program_vars (model_state.ST global_vars_list (program_map,cur_prog_name) fb_decl_list f_decl_list) =
-  (let st = (model_state.ST global_vars_list (program_map,cur_prog_name) fb_decl_list f_decl_list)
+definition initialize_program_vars :: "model_state \<Rightarrow> model_state" where
+"initialize_program_vars st  =
+  (case st of (model_state.ST global_vars_list (program_map,cur_prog_name) fb_decl_list f_decl_list) \<Rightarrow> 
+   (let st = (model_state.ST global_vars_list (program_map,cur_prog_name) fb_decl_list f_decl_list)
   in (model_state.ST 
     global_vars_list 
     (fmmap 
@@ -134,6 +139,69 @@ fun initialize_program_vars :: "model_state \<Rightarrow> model_state" where
        program_map,
       cur_prog_name) 
     fb_decl_list 
-    f_decl_list))"
+    f_decl_list)))"
+declare initialize_program_vars_def [simp]
+
+text "Initialization of global_vars"
+definition initialize_stacked_global_vars :: "model_state \<Rightarrow> stacked_global_vars \<Rightarrow> stacked_global_vars" where
+"initialize_stacked_global_vars st vars = 
+  (fmmap
+    (\<lambda>var. (case var of
+            stacked_global_var.Var val \<Rightarrow> stacked_global_var.Var (initialize_stacked_var st val)))
+    vars)"
+declare initialize_stacked_global_vars_def [simp]
+
+definition initialize_global_vars :: "model_state \<Rightarrow> model_state" where
+"initialize_global_vars st =
+  (case st of (model_state.ST global_vars (program_map,cur_prog_name) fb_decl_list f_decl_list) \<Rightarrow> 
+   (model_state.ST 
+    (initialize_stacked_global_vars st global_vars) 
+    (program_map,cur_prog_name) fb_decl_list f_decl_list))"
+
+text "Extracting new process state from stacked process"
+definition extract_process_state :: "stacked_process \<Rightarrow> process_state" where
+"extract_process_state sp  = 
+  (case sp of 
+    (proc_name, var_list,stst_list) \<Rightarrow> 
+    (let states = (map (\<lambda>(name,_,_,_). name) stst_list)
+      in (var_list, hd states, hd states, states, proc_status.Inactive, (time.Time 0 0 0 0 0))))"
+declare extract_process_state_def [simp]
+
+text "Extracting new program state from stacked program"
+definition extract_program_state :: "stacked_program \<Rightarrow> program_state" where 
+"extract_program_state sp =
+  (case sp of
+    (prog_name, var_list, st_proc_list) \<Rightarrow>
+      (let (name,_,_) = (nth st_proc_list 0);
+       proc_states = (fmap_of_list 
+                        (map 
+                          (\<lambda>(proc_name,var_list,state_list). 
+                            (proc_name,(extract_process_state (proc_name,var_list,state_list)))) 
+                          st_proc_list))
+    in (var_list,proc_states,name)))"
+declare extract_program_state_def [simp]
+
+text "Extracting new model state from stacked model"
+definition extract_model_state :: "stacked_model \<Rightarrow> model_state" where
+"extract_model_state sm =
+  (case sm of 
+    (conf, global, prog_list, fb_list, f_list) \<Rightarrow>
+(let (name, _, _) = (nth prog_list 0);
+        prog_map = (fmap_of_list
+    (map
+      (\<lambda>(name, var_list, proc_list). (name, (extract_program_state (name, var_list, proc_list))))
+      prog_list))
+  in (model_state.ST global (prog_map,name) fb_list f_list)))"
+declare extract_model_state_def [simp]
+
+definition initialize_model_state :: "stacked_model \<Rightarrow> model_state" where
+"initialize_model_state smodel = 
+  (let new_model = extract_model_state smodel;
+      m1 = initialize_global_vars new_model;
+      m2 = initialize_program_vars m1;
+      m3 = initialize_process_vars m2
+    in new_model)"
+declare initialize_model_state_def [simp]
+
 
 end
